Remove redundant assumption

pcuic/theories/PCUICSafeConversion.v
@@ -1695,7 +1695,7 @@ Section Conversion.
     eapply conv_context. eapply conv_App_r. assumption.
   Qed.
 
-  Lemma welltyped_it_mkLambda_or_LetIn :
+  Lemma welltyped_it_mkLambda_or_LetIn' :
     forall Γ t,
       ∥ wf_local Σ Γ ∥ ->
       welltyped Σ Γ t ->
@@ -1712,14 +1712,24 @@ Section Conversion.
       (* We don't have enough to conclude as B may only be a sort itself. *)
   Admitted.
 
+  Lemma welltyped_it_mkLambda_or_LetIn :
+    forall Γ t,
+      welltyped Σ Γ t ->
+      welltyped Σ [] (it_mkLambda_or_LetIn Γ t).
+  Proof.
+    intros Γ t h.
+    eapply welltyped_it_mkLambda_or_LetIn' ; try assumption.
+    destruct h as [A h]. constructor.
+    eapply typing_wf_local. eassumption.
+  Qed.
+
   Lemma welltyped_zipx :
     forall Γ t π,
-      ∥ wf_local Σ Γ ∥ ->
       welltyped Σ Γ (zipc t π) ->
       welltyped Σ [] (zipx Γ t π).
   Proof.
-    intros Γ t π hΓ h.
-    eapply welltyped_it_mkLambda_or_LetIn ; assumption.
+    intros Γ t π h.
+    eapply welltyped_it_mkLambda_or_LetIn. assumption.
   Qed.
 
   Equations _isconv (s : state) (Γ : context)
@@ -1736,12 +1746,12 @@ Section Conversion.
     _isconv Args Γ t π1 h1 π2 h2 aux :=
         _isconv_args Γ t π1 h1 π2 h2 aux.
 
-  Equations(noeqns) isconv_full (s : state) (Γ : context) (hΓ : ∥ wf_local Σ Γ ∥)
+  Equations(noeqns) isconv_full (s : state) (Γ : context)
             (t : term) (π1 : stack) (h1 : welltyped Σ Γ (zipc t π1))
             (π2 : stack) (h2 : wts Γ s t π2)
     : Ret s Γ t π1 π2 :=
 
-    isconv_full s Γ hΓ t π1 h1 π2 h2 :=
+    isconv_full s Γ t π1 h1 π2 h2 :=
       Fix_F (R := R)
             (fun '(s', Γ', t', π1', π2') => welltyped Σ Γ' (zipc t' π1') -> wts Γ' s' t' π2' -> Ret s' Γ' t' π1' π2')
             (fun t' f => _)
@@ -1758,16 +1768,16 @@ Section Conversion.
     eapply welltyped_zipx ; assumption.
   Qed.
 
-  Definition isconv Γ hΓ leq t1 π1 h1 t2 π2 h2 :=
-    let '(exist b _) := isconv_full (Reduction t2) Γ hΓ t1 π1 h1 π2 h2 leq in b.
+  Definition isconv Γ leq t1 π1 h1 t2 π2 h2 :=
+    let '(exist b _) := isconv_full (Reduction t2) Γ t1 π1 h1 π2 h2 leq in b.
 
   Theorem isconv_sound :
-    forall Γ hΓ leq t1 π1 h1 t2 π2 h2,
-      isconv Γ hΓ leq t1 π1 h1 t2 π2 h2 ->
+    forall Γ leq t1 π1 h1 t2 π2 h2,
+      isconv Γ leq t1 π1 h1 t2 π2 h2 ->
       conv leq Σ Γ (zipc t1 π1) (zipc t2 π2).
   Proof.
     unfold isconv.
-    intros Γ hΓ leq t1 π1 h1 t2 π2 h2.
+    intros Γ leq t1 π1 h1 t2 π2 h2.
     destruct isconv_full as [[]] ; auto.
     discriminate.
   Qed.
